Engine/PikeVM.v
@@ -6,7 +6,7 @@ Import ListNotations.
 From Linden Require Import Regex Chars Groups.
 From Linden Require Import Tree Semantics NFA.
 From Linden Require Import BooleanSemantics PikeSubset.
-From Warblre Require Import Base.
+From Warblre Require Import Base RegExpRecord.
 
 (** * PikeVM Semantics  *)
 (* exponential for now because we're not tracking the seen set yet *)
@@ -42,93 +42,98 @@ Inductive epsilon_result : Type :=
 
 Definition EpsDead : epsilon_result := EpsActive [].
 
-(* an atomic step for a thread *)
-Definition epsilon_step (t:thread) (c:code) (i:input): epsilon_result :=
-  match t with
-  | (pc, gm, b) =>
-      match get_pc c pc with
-      | None => EpsDead
-      | Some instr =>
-          match instr with
-          | Accept => EpsMatch
-          | Consume cd => match check_read cd i forward with
-                         | CannotRead => EpsDead
-                         | CanRead => EpsBlocked (block_thread t)
-                         end
-          | Jmp next => EpsActive [upd_label t next]
-          | Fork l1 l2 => EpsActive [upd_label t l1; upd_label t l2]
-          | SetRegOpen gid => EpsActive [open_thread t gid (idx i)]
-          | SetRegClose gid => EpsActive [close_thread t gid (idx i)]
-          | ResetRegs gidl => EpsActive [reset_thread t gidl]
-          | BeginLoop => EpsActive [begin_thread t]
-          | EndLoop next => match b with
-                           | CannotExit => EpsDead
-                           | CanExit => EpsActive [upd_label t next]
-                           end
-          | KillThread => EpsDead
-          end
-      end
-  end.
+Section PikeVM.
+  Context (rer: RegExpRecord).
 
-(* semantic states of the PikeVM algorithm *)
-Inductive pike_vm_state : Type :=
-| PVS (inp:input) (active: list thread) (best: option leaf) (blocked: list thread)
-| PVS_final (best: option leaf).
+  (* an atomic step for a thread *)
+  Definition epsilon_step (t:thread) (c:code) (i:input): epsilon_result :=
+    match t with
+    | (pc, gm, b) =>
+        match get_pc c pc with
+        | None => EpsDead
+        | Some instr =>
+            match instr with
+            | Accept => EpsMatch
+            | Consume cd => match check_read rer cd i forward with
+                          | CannotRead => EpsDead
+                          | CanRead => EpsBlocked (block_thread t)
+                          end
+            | Jmp next => EpsActive [upd_label t next]
+            | Fork l1 l2 => EpsActive [upd_label t l1; upd_label t l2]
+            | SetRegOpen gid => EpsActive [open_thread t gid (idx i)]
+            | SetRegClose gid => EpsActive [close_thread t gid (idx i)]
+            | ResetRegs gidl => EpsActive [reset_thread t gidl]
+            | BeginLoop => EpsActive [begin_thread t]
+            | EndLoop next => match b with
+                            | CannotExit => EpsDead
+                            | CanExit => EpsActive [upd_label t next]
+                            end
+            | KillThread => EpsDead
+            end
+        end
+    end.
 
-Definition pike_vm_initial_state (inp:input) : pike_vm_state :=
-  PVS inp [(0,GroupMap.empty,CanExit)] None [].
+  (* semantic states of the PikeVM algorithm *)
+  Inductive pike_vm_state : Type :=
+  | PVS (inp:input) (active: list thread) (best: option leaf) (blocked: list thread)
+  | PVS_final (best: option leaf).
 
-Definition gm_of (t:thread) : group_map :=
-  match t with (pc,gm,b) => gm end.
+  Definition pike_vm_initial_state (inp:input) : pike_vm_state :=
+    PVS inp [(0,GroupMap.empty,CanExit)] None [].
 
-(* small-tep semantics for the PikeVM algorithm *)
-Inductive pike_vm_step (c:code): pike_vm_state -> pike_vm_state -> Prop :=
-| pvs_final:
-(* moving to a final state when there are no more active or blocked threads *)
-  forall inp best,
-    pike_vm_step c (PVS inp [] best []) (PVS_final best)
-| pvs_end:
-  (* when the list of active is empty and we've reached the end of string *)
-  forall inp best blocked
-    (ADVANCE: advance_input inp forward = None),
-    pike_vm_step c (PVS inp [] best blocked) (PVS_final best)
-| pvs_nextchar:
-  (* when the list of active threads is empty (but not blocked), restart from the blocked ones, proceeding to the next character *)
-  forall inp1 inp2 best blocked thr
-    (ADVANCE: advance_input inp1 forward = Some inp2),
-    pike_vm_step c (PVS inp1 [] best (thr::blocked)) (PVS inp2 (thr::blocked) best [])
-| pvs_active:
-  (* generated new active threads: add them in front of the low-priority ones *)
-  forall inp t active best blocked nextactive
-    (STEP: epsilon_step t c inp = EpsActive nextactive),
-    pike_vm_step c (PVS inp (t::active) best blocked) (PVS inp (nextactive++active) best blocked)
-| pvs_match:
-  (* a match is found, discard remaining low-priority active threads *)
-  forall inp t active best blocked
-    (STEP: epsilon_step t c inp = EpsMatch),
-    pike_vm_step c (PVS inp (t::active) best blocked) (PVS inp [] (Some (inp, gm_of t)) blocked)
-| pvs_blocked:
-  (* add the new blocked thread after the previous ones *)
-  forall inp t active best blocked newt
-    (STEP: epsilon_step t c inp = EpsBlocked newt),
-    pike_vm_step c (PVS inp (t::active) best blocked) (PVS inp active best (blocked ++ [newt])).
+  Definition gm_of (t:thread) : group_map :=
+    match t with (pc,gm,b) => gm end.
 
-(** * PikeVM properties  *)
+  (* small-tep semantics for the PikeVM algorithm *)
+  Inductive pike_vm_step (c:code): pike_vm_state -> pike_vm_state -> Prop :=
+  | pvs_final:
+  (* moving to a final state when there are no more active or blocked threads *)
+    forall inp best,
+      pike_vm_step c (PVS inp [] best []) (PVS_final best)
+  | pvs_end:
+    (* when the list of active is empty and we've reached the end of string *)
+    forall inp best blocked
+      (ADVANCE: advance_input inp forward = None),
+      pike_vm_step c (PVS inp [] best blocked) (PVS_final best)
+  | pvs_nextchar:
+    (* when the list of active threads is empty (but not blocked), restart from the blocked ones, proceeding to the next character *)
+    forall inp1 inp2 best blocked thr
+      (ADVANCE: advance_input inp1 forward = Some inp2),
+      pike_vm_step c (PVS inp1 [] best (thr::blocked)) (PVS inp2 (thr::blocked) best [])
+  | pvs_active:
+    (* generated new active threads: add them in front of the low-priority ones *)
+    forall inp t active best blocked nextactive
+      (STEP: epsilon_step t c inp = EpsActive nextactive),
+      pike_vm_step c (PVS inp (t::active) best blocked) (PVS inp (nextactive++active) best blocked)
+  | pvs_match:
+    (* a match is found, discard remaining low-priority active threads *)
+    forall inp t active best blocked
+      (STEP: epsilon_step t c inp = EpsMatch),
+      pike_vm_step c (PVS inp (t::active) best blocked) (PVS inp [] (Some (inp, gm_of t)) blocked)
+  | pvs_blocked:
+    (* add the new blocked thread after the previous ones *)
+    forall inp t active best blocked newt
+      (STEP: epsilon_step t c inp = EpsBlocked newt),
+      pike_vm_step c (PVS inp (t::active) best blocked) (PVS inp active best (blocked ++ [newt])).
 
-Theorem pikevm_deterministic:
-  forall c pvso pvs1 pvs2
-    (STEP1: pike_vm_step c pvso pvs1)
-    (STEP2: pike_vm_step c pvso pvs2),
-    pvs1 = pvs2.
-Proof.
-  intros c pvso pvs1 pvs2 STEP1 STEP2. inversion STEP1; subst.
-  - inversion STEP2; subst; auto. 
-  - inversion STEP2; subst; auto. rewrite ADVANCE in ADVANCE0; inversion ADVANCE0.
-  - inversion STEP2; subst; auto; rewrite ADVANCE in ADVANCE0; inversion ADVANCE0.
-    subst. auto.
-  - inversion STEP2; subst; auto; rewrite STEP in STEP0; inversion STEP0.
-    subst. auto.
-  - inversion STEP2; subst; auto; rewrite STEP in STEP0; inversion STEP0.
-  - inversion STEP2; subst; auto; rewrite STEP in STEP0; inversion STEP0.
-    subst. auto.
-Qed.
+  (** * PikeVM properties  *)
+
+  Theorem pikevm_deterministic:
+    forall c pvso pvs1 pvs2
+      (STEP1: pike_vm_step c pvso pvs1)
+      (STEP2: pike_vm_step c pvso pvs2),
+      pvs1 = pvs2.
+  Proof.
+    intros c pvso pvs1 pvs2 STEP1 STEP2. inversion STEP1; subst.
+    - inversion STEP2; subst; auto. 
+    - inversion STEP2; subst; auto. rewrite ADVANCE in ADVANCE0; inversion ADVANCE0.
+    - inversion STEP2; subst; auto; rewrite ADVANCE in ADVANCE0; inversion ADVANCE0.
+      subst. auto.
+    - inversion STEP2; subst; auto; rewrite STEP in STEP0; inversion STEP0.
+      subst. auto.
+    - inversion STEP2; subst; auto; rewrite STEP in STEP0; inversion STEP0.
+    - inversion STEP2; subst; auto; rewrite STEP in STEP0; inversion STEP0.
+      subst. auto.
+  Qed.
+
+End PikeVM.
